src/basic/FStarC.Options.fst
@@ -222,6 +222,7 @@ let defaults = [
   ("fuel"                                      , Unset);
   ("help"                                      , Bool false);
   ("hide_uvar_nums"                            , Bool false);
+  ("html"                                      , Bool false);
   ("hint_dir"                                  , Unset);
   ("hint_file"                                 , Unset);
   ("hint_hook"                                 , Unset);
@@ -487,6 +488,7 @@ let get_extract_namespace       ()      = lookup_opt "extract_namespace"        
 let get_force                   ()      = lookup_opt "force"                    as_bool
 let get_help                    ()      = lookup_opt "help"                     as_bool
 let get_hide_uvar_nums          ()      = lookup_opt "hide_uvar_nums"           as_bool
+let get_html                    ()      = lookup_opt "html"                     as_bool
 let get_hint_info               ()      = lookup_opt "hint_info"                as_bool
 let get_hint_dir                ()      = lookup_opt "hint_dir"                 (as_option as_string)
 let get_hint_file               ()      = lookup_opt "hint_file"                (as_option as_string)
@@ -1011,6 +1013,11 @@ let specs_with_types warn_unsafe : ML (list (char & string & opt_type & Pprint.d
     "hide_uvar_nums",
     Const (Bool true),
     text "Don't print unification variable numbers");
+
+  ( noshort,
+    "html",
+    Const (Bool true),
+    text "Generate syntax-highlighted HTML with cross-reference links for input files");
 
   ( noshort,
     "hint_dir",
@@ -2096,6 +2103,7 @@ let hint_file_for_src src_filename =
           | _ -> src_filename
         in
         Format.fmt1 "%s.hints" file_name
+let html                         () = get_html                        ()
 let ide                          () = get_ide                         ()
 let ide_id_info_off              () = get_ide_id_info_off             ()
 let ide_file_name_st =
